<?xml version="1.0"?>
<rdf:RDF xmlns="http://purl.obolibrary.org/obo/cpo.owl#"
     xml:base="http://purl.obolibrary.org/obo/cpo.owl"
     xmlns:owl="http://www.w3.org/2002/07/owl#"
     xmlns:oboInOwl="http://www.geneontology.org/formats/oboInOwl#"
     xmlns:protege="http://protege.stanford.edu/plugins/owl/protege#"
     xmlns:xsd="http://www.w3.org/2001/XMLSchema#"
     xmlns:rdfs="http://www.w3.org/2000/01/rdf-schema#"
     xmlns:cito="http://purl.org/spar/cito/"
     xmlns:swrla="http://swrl.stanford.edu/ontologies/3.3/swrla.owl#"
     xmlns:rdf="http://www.w3.org/1999/02/22-rdf-syntax-ns#"
     xmlns:terms="http://purl.org/dc/terms/"
     xmlns:xml="http://www.w3.org/XML/1998/namespace"
     xmlns:oboInOwl1="ttp://www.geneontology.org/formats/oboInOwl#"
     xmlns:obo="http://purl.obolibrary.org/obo/"
     xmlns:foaf="http://xmlns.com/foaf/0.1/"
     xmlns:dc="http://purl.org/dc/elements/1.1/"
     xmlns:subsets="http://purl.obolibrary.org/obo/ro/subsets#">
    <owl:Ontology rdf:about="http://purl.obolibrary.org/obo/cpo.owl">
        <owl:versionIRI rdf:resource="http://purl.obolibrary.org/obo/2018-09-24/cpo.owl"/>
        <owl:imports rdf:resource="http://purl.obolibrary.org/obo/ro/releases/2018-05-11/ro.owl"/>
        <owl:imports rdf:resource="http://purl.obolibrary.org/obo/iao/2017-03-24/iao.owl"/>
        <dc:description xml:lang="en">This ontology has been designed to conform to BFO and OBO standards and stands in reference to the following works (non-exhaustive):

Lewis, Cara C., Predrag Klasnja, Byron J. Powell, Aaron R. Lyon, Leah Tuzzio, Salene Jones, Callie Walsh-Bailey, and Bryan Weiner. “From Classification to Causality: Advancing Understanding of Mechanisms of Change in Implementation Science.” Frontiers in Public Health 6 (2018). https://doi.org/10.3389/fpubh.2018.00136.

Michie, Susan, Stefanie Ashford, Falko F. Sniehotta, Stephan U. Dombrowski, Alex Bishop, and David P. French. “A Refined Taxonomy of Behaviour Change Techniques to Help People Change Their Physical Activity and Healthy Eating Behaviours: The CALO-RE Taxonomy.” Psychology &amp; Health 26, no. 11 (November 1, 2011): 1479–98. https://doi.org/10.1080/08870446.2010.540664.

More publication citations can be found at the annotation property level for the interested reader.</dc:description>
        <dc:creator xml:lang="en">John Rincon</dc:creator>
        <dc:creator xml:lang="en">Cooper Stansbury</dc:creator>
        <owl:versionInfo xml:lang="en">1.0.0</owl:versionInfo>
        <dc:creator xml:lang="en">Zach Landis-Lewis</dc:creator>
        <dc:title xml:lang="en">Causal Pathway Ontology</dc:title>
        <terms:license xml:lang="en">https://creativecommons.org/licenses/by/4.0/</terms:license>
        <dc:creator xml:lang="en">Colin Gross</dc:creator>
    </owl:Ontology>
    


    <!-- 
    ///////////////////////////////////////////////////////////////////////////////////////
    //
    // Classes
    //
    ///////////////////////////////////////////////////////////////////////////////////////
     -->

    


    <!-- http://purl.obolibrary.org/obo/cpo_0000001 -->

    <owl:Class rdf:about="http://purl.obolibrary.org/obo/cpo_0000001">
        <rdfs:subClassOf rdf:resource="http://purl.obolibrary.org/obo/cpo_0000004"/>
        <obo:IAO_0000115 xml:lang="en">A mediator through which an implementation strategy operates to affect desired implementation outcomes.</obo:IAO_0000115>
        <obo:IAO_0000117 xml:lang="en">Cooper Stansbury</obo:IAO_0000117>
        <obo:IAO_0000119 xml:lang="en">Lewis CC, Klasnja P, Powell BJ, Lyon AR, Tuzzio L, Jones S, et al. From Classification to Causality: Advancing Understanding of Mechanisms of Change in Implementation Science. Front Public Health [Internet]. 2018 [cited 2018 Jun 6];6. Available from: https://www.frontiersin.org/articles/10.3389/fpubh.2018.00136/full</obo:IAO_0000119>
        <obo:IAO_0000232 xml:lang="en">This definition needs work. it is unclear how the authors of the cited source intend the relationship between moderators and mediators, given that they are not both defined as subclasses with a common parent.</obo:IAO_0000232>
        <rdfs:label xml:lang="en">mechanism</rdfs:label>
    </owl:Class>
    


    <!-- http://purl.obolibrary.org/obo/cpo_0000002 -->

    <owl:Class rdf:about="http://purl.obolibrary.org/obo/cpo_0000002">
        <rdfs:subClassOf rdf:resource="http://purl.obolibrary.org/obo/IAO_0000030"/>
        <obo:IAO_0000115 xml:lang="en">An information content entity that is necessary for a mechanism or implementation outcome to be activated.</obo:IAO_0000115>
        <obo:IAO_0000117 xml:lang="en">Cooper Stansbury</obo:IAO_0000117>
        <obo:IAO_0000119 xml:lang="en">Lewis CC, Klasnja P, Powell BJ, Lyon AR, Tuzzio L, Jones S, et al. From Classification to Causality: Advancing Understanding of Mechanisms of Change in Implementation Science. Front Public Health [Internet]. 2018 [cited 2018 Jun 6];6. Available from: https://www.frontiersin.org/articles/10.3389/fpubh.2018.00136/full</obo:IAO_0000119>
        <rdfs:label xml:lang="en">precondition</rdfs:label>
    </owl:Class>
    


    <!-- http://purl.obolibrary.org/obo/cpo_0000003 -->

    <owl:Class rdf:about="http://purl.obolibrary.org/obo/cpo_0000003">
        <rdfs:subClassOf rdf:resource="http://www.geneontology.org/formats/oboInOwl#ObsoleteClass"/>
        <obo:IAO_0000115 xml:lang="en">A contextual factor that enables or hinders the implementation strategy from eliciting the desired effect.</obo:IAO_0000115>
        <obo:IAO_0000117 xml:lang="en">Cooper Stansbury</obo:IAO_0000117>
        <obo:IAO_0000119 xml:lang="en">Lewis CC, Klasnja P, Powell BJ, Lyon AR, Tuzzio L, Jones S, et al. From Classification to Causality: Advancing Understanding of Mechanisms of Change in Implementation Science. Front Public Health [Internet]. 2018 [cited 2018 Jun 6];6. Available from: https://www.frontiersin.org/articles/10.3389/fpubh.2018.00136/full</obo:IAO_0000119>
        <obo:IAO_0000232 xml:lang="en">Also referred to as “barriers” and “facilitators”</obo:IAO_0000232>
        <rdfs:label rdf:datatype="http://www.w3.org/2001/XMLSchema#string">obsolete determinant</rdfs:label>
        <owl:deprecated rdf:datatype="http://www.w3.org/2001/XMLSchema#boolean">true</owl:deprecated>
    </owl:Class>
    


    <!-- http://purl.obolibrary.org/obo/cpo_0000004 -->

    <owl:Class rdf:about="http://purl.obolibrary.org/obo/cpo_0000004">
        <rdfs:subClassOf rdf:resource="http://purl.obolibrary.org/obo/IAO_0000030"/>
        <obo:IAO_0000115 xml:lang="en">An information content entity that may account for the relationship between the implementation strategy and the implementation outcome.</obo:IAO_0000115>
        <obo:IAO_0000117 xml:lang="en">Cooper Stansbury</obo:IAO_0000117>
        <obo:IAO_0000119 xml:lang="en">Lewis CC, Klasnja P, Powell BJ, Lyon AR, Tuzzio L, Jones S, et al. From Classification to Causality: Advancing Understanding of Mechanisms of Change in Implementation Science. Front Public Health [Internet]. 2018 [cited 2018 Jun 6];6. Available from: https://www.frontiersin.org/articles/10.3389/fpubh.2018.00136/full</obo:IAO_0000119>
        <rdfs:label xml:lang="en">mediator</rdfs:label>
    </owl:Class>
    


    <!-- http://purl.obolibrary.org/obo/cpo_0000005 -->

    <owl:Class rdf:about="http://purl.obolibrary.org/obo/cpo_0000005">
        <rdfs:subClassOf rdf:resource="http://purl.obolibrary.org/obo/IAO_0000030"/>
        <obo:IAO_0000115 xml:lang="en">An information content entity that may affect the level of influence of an implementation strategy.</obo:IAO_0000115>
        <obo:IAO_0000117 xml:lang="en">Cooper Stansbury</obo:IAO_0000117>
        <obo:IAO_0000119 xml:lang="en">Lewis CC, Klasnja P, Powell BJ, Lyon AR, Tuzzio L, Jones S, et al. From Classification to Causality: Advancing Understanding of Mechanisms of Change in Implementation Science. Front Public Health [Internet]. 2018 [cited 2018 Jun 6];6. Available from: https://www.frontiersin.org/articles/10.3389/fpubh.2018.00136/full</obo:IAO_0000119>
        <obo:IAO_0000232 xml:lang="en">moderators functionally &apos;act&apos; on mechanisms, but do not prevent or require mechanisms to &apos;fire.&apos;</obo:IAO_0000232>
        <rdfs:label xml:lang="en">moderator</rdfs:label>
    </owl:Class>
    


    <!-- http://purl.obolibrary.org/obo/cpo_0000006 -->

    <owl:Class rdf:about="http://purl.obolibrary.org/obo/cpo_0000006">
        <rdfs:subClassOf rdf:resource="http://purl.obolibrary.org/obo/IAO_0000030"/>
        <obo:IAO_0000115 xml:lang="en">An information content entity that represents the outcome of the implementation strategy that is realized because of its specific mechanism of action, and is the most immediate, observable outcome in the causal pathway.</obo:IAO_0000115>
        <obo:IAO_0000117 xml:lang="en">Cooper Stansbury</obo:IAO_0000117>
        <obo:IAO_0000119 xml:lang="en">Lewis CC, Klasnja P, Powell BJ, Lyon AR, Tuzzio L, Jones S, et al. From Classification to Causality: Advancing Understanding of Mechanisms of Change in Implementation Science. Front Public Health [Internet]. 2018 [cited 2018 Jun 6];6. Available from: https://www.frontiersin.org/articles/10.3389/fpubh.2018.00136/full</obo:IAO_0000119>
        <rdfs:label xml:lang="en">proximal outcome</rdfs:label>
    </owl:Class>
    


    <!-- http://purl.obolibrary.org/obo/cpo_0000007 -->

    <owl:Class rdf:about="http://purl.obolibrary.org/obo/cpo_0000007">
        <rdfs:subClassOf rdf:resource="http://purl.obolibrary.org/obo/IAO_0000030"/>
        <obo:IAO_0000115 xml:lang="en">An information content entity that represents the outcome that a candidate intervention is designed to achieve.</obo:IAO_0000115>
        <obo:IAO_0000117 xml:lang="en">Cooper Stansbury</obo:IAO_0000117>
        <obo:IAO_0000119 xml:lang="en">Lewis CC, Klasnja P, Powell BJ, Lyon AR, Tuzzio L, Jones S, et al. From Classification to Causality: Advancing Understanding of Mechanisms of Change in Implementation Science. Front Public Health [Internet]. 2018 [cited 2018 Jun 6];6. Available from: https://www.frontiersin.org/articles/10.3389/fpubh.2018.00136/full</obo:IAO_0000119>
        <rdfs:label xml:lang="en">distal outcome</rdfs:label>
    </owl:Class>
    


    <!-- http://purl.obolibrary.org/obo/cpo_0000008 -->

    <owl:Class rdf:about="http://purl.obolibrary.org/obo/cpo_0000008">
        <rdfs:subClassOf rdf:resource="http://purl.obolibrary.org/obo/cpo_0000005"/>
        <obo:IAO_0000115 xml:lang="en">A moderator that affects the level of influence of an implementation strategy before a mechanism acts on the situation.</obo:IAO_0000115>
        <obo:IAO_0000117 xml:lang="en">Cooper Stansbury</obo:IAO_0000117>
        <obo:IAO_0000119 xml:lang="en">Lewis CC, Klasnja P, Powell BJ, Lyon AR, Tuzzio L, Jones S, et al. From Classification to Causality: Advancing Understanding of Mechanisms of Change in Implementation Science. Front Public Health [Internet]. 2018 [cited 2018 Jun 6];6. Available from: https://www.frontiersin.org/articles/10.3389/fpubh.2018.00136/full</obo:IAO_0000119>
        <obo:IAO_0000232 xml:lang="en">the authors of the cited source are unclear concerning the definitive difference between &apos;cognitive&apos; and &apos;organizational&apos; moderators except in the diagrams on page 3. The indicates a temporal difference between the two, which has been represented here.</obo:IAO_0000232>
        <rdfs:label xml:lang="en">cognitive moderator</rdfs:label>
    </owl:Class>
    


    <!-- http://purl.obolibrary.org/obo/cpo_0000009 -->

    <owl:Class rdf:about="http://purl.obolibrary.org/obo/cpo_0000009">
        <rdfs:subClassOf rdf:resource="http://purl.obolibrary.org/obo/cpo_0000005"/>
        <obo:IAO_0000115 xml:lang="en">A moderator that affects the level of influence of an implementation strategy after, or simultaneously with, a mechanism that acts on the situation.</obo:IAO_0000115>
        <obo:IAO_0000117 xml:lang="en">Cooper Stansbury</obo:IAO_0000117>
        <obo:IAO_0000119 xml:lang="en">Lewis CC, Klasnja P, Powell BJ, Lyon AR, Tuzzio L, Jones S, et al. From Classification to Causality: Advancing Understanding of Mechanisms of Change in Implementation Science. Front Public Health [Internet]. 2018 [cited 2018 Jun 6];6. Available from: https://www.frontiersin.org/articles/10.3389/fpubh.2018.00136/full</obo:IAO_0000119>
        <rdfs:label xml:lang="en">organizational moderator</rdfs:label>
    </owl:Class>
    


    <!-- http://purl.obolibrary.org/obo/cpo_0000010 -->

    <owl:Class rdf:about="http://purl.obolibrary.org/obo/cpo_0000010">
        <rdfs:subClassOf rdf:resource="http://www.geneontology.org/formats/oboInOwl#ObsoleteClass"/>
        <obo:IAO_0000115 xml:lang="en">A directive information entity that prescribes a procedure to achieve a specified outcome in an intervention.</obo:IAO_0000115>
        <obo:IAO_0000116 xml:lang="en">Secondary definition: the methods or techniques used to enhance the adoption, implementation, and sustainability of a program or practice.

From: Pai et al., “Strategies to Enhance Venous Thromboprophylaxis in Hospitalized Medical Patients (SENTRY).”</obo:IAO_0000116>
        <obo:IAO_0000117 xml:lang="en">Cooper Stansbury</obo:IAO_0000117>
        <obo:IAO_0000119 xml:lang="en">Mazza et al., “Refining a Taxonomy for Guideline Implementation.”</obo:IAO_0000119>
        <obo:IAO_0000232 xml:lang="en">Many of the subclasses for this term were taken as-is from “EPOC Taxonomy | Cochrane Effective Practice and Organisation of Care.” The complete taxomony structure was not taken. Need to revisit.</obo:IAO_0000232>
        <rdfs:label rdf:datatype="http://www.w3.org/2001/XMLSchema#string">obsolete implementation strategy</rdfs:label>
        <owl:deprecated rdf:datatype="http://www.w3.org/2001/XMLSchema#boolean">true</owl:deprecated>
    </owl:Class>
    


    <!-- http://purl.obolibrary.org/obo/cpo_0000011 -->

    <owl:Class rdf:about="http://purl.obolibrary.org/obo/cpo_0000011">
        <rdfs:subClassOf rdf:resource="http://www.geneontology.org/formats/oboInOwl#ObsoleteClass"/>
        <obo:IAO_0000115 xml:lang="en">A process of intervening on people, groups, entities or objects in an experimental study.</obo:IAO_0000115>
        <obo:IAO_0000117 xml:lang="en">Cooper Stansbury</obo:IAO_0000117>
        <obo:IAO_0000119 xml:lang="en">“Glossary | Cochrane Community.”</obo:IAO_0000119>
        <obo:IAO_0000232 xml:lang="en">In controlled trials, the word is sometimes used to describe the regimens in all comparison groups, including placebo and no-treatment arms</obo:IAO_0000232>
        <rdfs:label rdf:datatype="http://www.w3.org/2001/XMLSchema#string">obsolete intervention</rdfs:label>
        <owl:deprecated rdf:datatype="http://www.w3.org/2001/XMLSchema#boolean">true</owl:deprecated>
    </owl:Class>
    


    <!-- http://purl.obolibrary.org/obo/cpo_0000013 -->

    <owl:Class rdf:about="http://purl.obolibrary.org/obo/cpo_0000013">
        <rdfs:subClassOf rdf:resource="http://www.geneontology.org/formats/oboInOwl#ObsoleteClass"/>
        <obo:IAO_0000115 xml:lang="en">A generically dependent continuant which is the conditions and circumstances that are relevant to the application of an intervention.</obo:IAO_0000115>
        <obo:IAO_0000117 xml:lang="en">Cooper Stansbury</obo:IAO_0000117>
        <obo:IAO_0000119 xml:lang="en">“Glossary | Cochrane Community.”</obo:IAO_0000119>
        <obo:IAO_0000232 xml:lang="en">for example the setting (in hospital, at home, in the air); the time (working day, holiday, night-time); type of practice (primary, secondary, tertiary care; private practice, insurance practice, charity); whether routine or emergency</obo:IAO_0000232>
        <rdfs:label rdf:datatype="http://www.w3.org/2001/XMLSchema#string">obsolete context</rdfs:label>
        <owl:deprecated rdf:datatype="http://www.w3.org/2001/XMLSchema#boolean">true</owl:deprecated>
    </owl:Class>
    


    <!-- http://purl.obolibrary.org/obo/cpo_0000014 -->

    <owl:Class rdf:about="http://purl.obolibrary.org/obo/cpo_0000014">
        <rdfs:subClassOf rdf:resource="http://www.geneontology.org/formats/oboInOwl#ObsoleteClass"/>
        <obo:IAO_0000115 xml:lang="en">A specifically dependent continuant which is the extent to which a specific intervention, when used under ordinary circumstances, does what it is intended to do.</obo:IAO_0000115>
        <obo:IAO_0000117 xml:lang="en">Cooper Stansbury</obo:IAO_0000117>
        <obo:IAO_0000119 xml:lang="en">“Glossary | Cochrane Community.”</obo:IAO_0000119>
        <rdfs:label rdf:datatype="http://www.w3.org/2001/XMLSchema#string">obsolete effectiveness</rdfs:label>
        <owl:deprecated rdf:datatype="http://www.w3.org/2001/XMLSchema#boolean">true</owl:deprecated>
    </owl:Class>
    


    <!-- http://purl.obolibrary.org/obo/cpo_0000016 -->

    <owl:Class rdf:about="http://purl.obolibrary.org/obo/cpo_0000016">
        <rdfs:subClassOf rdf:resource="http://www.geneontology.org/formats/oboInOwl#ObsoleteClass"/>
        <obo:IAO_0000115 xml:lang="en">A process which is a component of a recipient&apos;s status after an intervention has been applied that is used to assess the effectiveness of an intervention.</obo:IAO_0000115>
        <obo:IAO_0000117 xml:lang="en">Cooper Stansbury</obo:IAO_0000117>
        <obo:IAO_0000119 xml:lang="en">“Glossary | Cochrane Community.”</obo:IAO_0000119>
        <rdfs:label rdf:datatype="http://www.w3.org/2001/XMLSchema#string">obsolete intervention outcome</rdfs:label>
        <owl:deprecated rdf:datatype="http://www.w3.org/2001/XMLSchema#boolean">true</owl:deprecated>
    </owl:Class>
    


    <!-- http://purl.obolibrary.org/obo/cpo_0000017 -->

    <owl:Class rdf:about="http://purl.obolibrary.org/obo/cpo_0000017">
        <rdfs:subClassOf rdf:resource="http://www.geneontology.org/formats/oboInOwl#ObsoleteClass"/>
        <obo:IAO_0000115 xml:lang="en">Strategies to change organisational culture.</obo:IAO_0000115>
        <obo:IAO_0000117 xml:lang="en">Cooper Stansbury</obo:IAO_0000117>
        <obo:IAO_0000119 xml:lang="en">“EPOC Taxonomy | Cochrane Effective Practice and Organisation of Care.”</obo:IAO_0000119>
        <rdfs:label rdf:datatype="http://www.w3.org/2001/XMLSchema#string">obsolete organisational culture</rdfs:label>
        <owl:deprecated rdf:datatype="http://www.w3.org/2001/XMLSchema#boolean">true</owl:deprecated>
    </owl:Class>
    


    <!-- http://purl.obolibrary.org/obo/cpo_0000018 -->

    <owl:Class rdf:about="http://purl.obolibrary.org/obo/cpo_0000018">
        <rdfs:subClassOf rdf:resource="http://www.geneontology.org/formats/oboInOwl#ObsoleteClass"/>
        <obo:IAO_0000115 xml:lang="en">A summary of health workers’ performance over a specified period of time, given to them in a written electronic or verbal format. The summary may include recommendations for clinical action</obo:IAO_0000115>
        <obo:IAO_0000117 xml:lang="en">Cooper Stansbury</obo:IAO_0000117>
        <obo:IAO_0000119 xml:lang="en">“EPOC Taxonomy | Cochrane Effective Practice and Organisation of Care.”</obo:IAO_0000119>
        <rdfs:label rdf:datatype="http://www.w3.org/2001/XMLSchema#string">obsolete audit and feedback</rdfs:label>
        <owl:deprecated rdf:datatype="http://www.w3.org/2001/XMLSchema#boolean">true</owl:deprecated>
    </owl:Class>
    


    <!-- http://purl.obolibrary.org/obo/cpo_0000019 -->

    <owl:Class rdf:about="http://purl.obolibrary.org/obo/cpo_0000019">
        <rdfs:subClassOf rdf:resource="http://www.geneontology.org/formats/oboInOwl#ObsoleteClass"/>
        <obo:IAO_0000115 xml:lang="en">Monitoring of health services by individuals or healthcare organisations, for example by comparing with an external standard.</obo:IAO_0000115>
        <obo:IAO_0000117 xml:lang="en">Cooper Stansbury</obo:IAO_0000117>
        <rdfs:label rdf:datatype="http://www.w3.org/2001/XMLSchema#string">obsolete monitoring the performance of the delivery of healthcare</rdfs:label>
        <owl:deprecated rdf:datatype="http://www.w3.org/2001/XMLSchema#boolean">true</owl:deprecated>
    </owl:Class>
    


    <!-- http://purl.obolibrary.org/obo/cpo_0000020 -->

    <owl:Class rdf:about="http://purl.obolibrary.org/obo/cpo_0000020">
        <rdfs:subClassOf rdf:resource="http://www.geneontology.org/formats/oboInOwl#ObsoleteClass"/>
        <obo:IAO_0000115 xml:lang="en">An iterative process to review and improve care that includes involvement of healthcare teams, analysis of a process or system, a structured process improvement method or problem solving approach, and use of data analysis to assess changes</obo:IAO_0000115>
        <obo:IAO_0000117 xml:lang="en">Cooper Stansbury</obo:IAO_0000117>
        <rdfs:label rdf:datatype="http://www.w3.org/2001/XMLSchema#string">obsolete continuous quality improvement</rdfs:label>
        <owl:deprecated rdf:datatype="http://www.w3.org/2001/XMLSchema#boolean">true</owl:deprecated>
    </owl:Class>
    


    <!-- http://purl.obolibrary.org/obo/cpo_0000021 -->

    <owl:Class rdf:about="http://purl.obolibrary.org/obo/cpo_0000021">
        <rdfs:subClassOf rdf:resource="http://www.geneontology.org/formats/oboInOwl#ObsoleteClass"/>
        <obo:IAO_0000115 xml:lang="en">Interventions to change practice that are selected based on an assessment of barriers to change, for example through interviews or surveys</obo:IAO_0000115>
        <obo:IAO_0000117 xml:lang="en">Cooper Stansbury</obo:IAO_0000117>
        <obo:IAO_0000119 xml:lang="en">“EPOC Taxonomy | Cochrane Effective Practice and Organisation of Care.”</obo:IAO_0000119>
        <rdfs:label rdf:datatype="http://www.w3.org/2001/XMLSchema#string">obsolete tailored interventions</rdfs:label>
        <owl:deprecated rdf:datatype="http://www.w3.org/2001/XMLSchema#boolean">true</owl:deprecated>
    </owl:Class>
    


    <!-- http://purl.obolibrary.org/obo/cpo_0000023 -->

    <owl:Class rdf:about="http://purl.obolibrary.org/obo/cpo_0000023">
        <rdfs:subClassOf rdf:resource="http://www.geneontology.org/formats/oboInOwl#ObsoleteClass"/>
        <obo:IAO_0000115 xml:lang="en">A mechanism that affects the ability to focus selectively on aspects of the environment.</obo:IAO_0000115>
        <obo:IAO_0000117 xml:lang="en">Cooper Stansbury</obo:IAO_0000117>
        <obo:IAO_0000119 xml:lang="en">Cane J, O’Connor D, Michie S. Validation of the theoretical domains framework for use in behaviour change and implementation research. Implementation Science. 2012 Apr 24;7:37.</obo:IAO_0000119>
        <rdfs:label rdf:datatype="http://www.w3.org/2001/XMLSchema#string">obsolete act on attention</rdfs:label>
        <owl:deprecated rdf:datatype="http://www.w3.org/2001/XMLSchema#boolean">true</owl:deprecated>
    </owl:Class>
    


    <!-- http://purl.obolibrary.org/obo/cpo_0000024 -->

    <owl:Class rdf:about="http://purl.obolibrary.org/obo/cpo_0000024">
        <rdfs:subClassOf rdf:resource="http://www.geneontology.org/formats/oboInOwl#ObsoleteClass"/>
        <obo:IAO_0000115 xml:lang="en">A mechanism that affects acceptance of the truth, reality, or validity about an ability, talent, or facility that a person can put to constructive use.</obo:IAO_0000115>
        <obo:IAO_0000117 xml:lang="en">Cooper Stansbury</obo:IAO_0000117>
        <obo:IAO_0000119 xml:lang="en">Cane J, O’Connor D, Michie S. Validation of the theoretical domains framework for use in behaviour change and implementation research. Implementation Science. 2012 Apr 24;7:37.</obo:IAO_0000119>
        <obo:IAO_0000119 xml:lang="en">Kolehmainen N, Francis JJ. Specifying content and mechanisms of change in interventions to change professionals’ practice: an illustration from the Good Goals study in occupational therapy. Implementation Science. 2012 Oct 18;7:100.</obo:IAO_0000119>
        <rdfs:label rdf:datatype="http://www.w3.org/2001/XMLSchema#string">obsolete act on belief about capabilities</rdfs:label>
        <owl:deprecated rdf:datatype="http://www.w3.org/2001/XMLSchema#boolean">true</owl:deprecated>
    </owl:Class>
    


    <!-- http://purl.obolibrary.org/obo/cpo_0000025 -->

    <owl:Class rdf:about="http://purl.obolibrary.org/obo/cpo_0000025">
        <rdfs:subClassOf rdf:resource="http://www.geneontology.org/formats/oboInOwl#ObsoleteClass"/>
        <obo:IAO_0000115 xml:lang="en">A mechanism that affects a complex reaction pattern, involving experiential, behavioural, and physiological elements, by which the individual attempts to deal with a personally significant matter or event.</obo:IAO_0000115>
        <obo:IAO_0000117 xml:lang="en">Cooper Stansbury</obo:IAO_0000117>
        <obo:IAO_0000119 xml:lang="en">Cane J, O’Connor D, Michie S. Validation of the theoretical domains framework for use in behaviour change and implementation research. Implementation Science. 2012 Apr 24;7:37.</obo:IAO_0000119>
        <obo:IAO_0000119 xml:lang="en">Kolehmainen N, Francis JJ. Specifying content and mechanisms of change in interventions to change professionals’ practice: an illustration from the Good Goals study in occupational therapy. Implementation Science. 2012 Oct 18;7:100.</obo:IAO_0000119>
        <rdfs:label rdf:datatype="http://www.w3.org/2001/XMLSchema#string">obsolete act on emotion</rdfs:label>
        <owl:deprecated rdf:datatype="http://www.w3.org/2001/XMLSchema#boolean">true</owl:deprecated>
    </owl:Class>
    


    <!-- http://purl.obolibrary.org/obo/cpo_0000029 -->

    <owl:Class rdf:about="http://purl.obolibrary.org/obo/cpo_0000029">
        <rdfs:subClassOf rdf:resource="http://purl.obolibrary.org/obo/IAO_0000030"/>
        <obo:IAO_0000115 xml:lang="en">An information content entity about a process through which an implementation strategy operates to affect desired implementation outcomes.</obo:IAO_0000115>
        <obo:IAO_0000117 xml:lang="en">Cooper Stansbury</obo:IAO_0000117>
        <obo:IAO_0000119 xml:lang="en">Lewis CC, Klasnja P, Powell BJ, Lyon AR, Tuzzio L, Jones S, et al. From Classification to Causality: Advancing Understanding of Mechanisms of Change in Implementation Science. Front Public Health [Internet]. 2018 [cited 2018 Jun 6];6. Available from: https://www.frontiersin.org/articles/10.3389/fpubh.2018.00136/full</obo:IAO_0000119>
        <obo:IAO_0000232 xml:lang="en">A causal pathway is a set of features &quot;of the mechanistic processes through which implementation strategies operate&quot; (Lewis 2018).</obo:IAO_0000232>
        <rdfs:label xml:lang="en">causal pathway</rdfs:label>
    </owl:Class>
    


    <!-- http://purl.obolibrary.org/obo/cpo_0000030 -->

    <owl:Class rdf:about="http://purl.obolibrary.org/obo/cpo_0000030">
        <rdfs:subClassOf rdf:resource="http://www.geneontology.org/formats/oboInOwl#ObsoleteClass"/>
        <obo:IAO_0000115 xml:lang="en">A precondition that allows for the possibility of a mechanism to act</obo:IAO_0000115>
        <obo:IAO_0000117 xml:lang="en">Cooper Stansbury</obo:IAO_0000117>
        <obo:IAO_0000119 xml:lang="en">Lewis CC, Klasnja P, Powell BJ, Lyon AR, Tuzzio L, Jones S, et al. From Classification to Causality: Advancing Understanding of Mechanisms of Change in Implementation Science. Front Public Health [Internet]. 2018 [cited 2018 Jun 6];6. Available from: https://www.frontiersin.org/articles/10.3389/fpubh.2018.00136/full</obo:IAO_0000119>
        <rdfs:label rdf:datatype="http://www.w3.org/2001/XMLSchema#string">obsolete precondition for mechanism of activation</rdfs:label>
        <owl:deprecated rdf:datatype="http://www.w3.org/2001/XMLSchema#boolean">true</owl:deprecated>
    </owl:Class>
    


    <!-- http://purl.obolibrary.org/obo/cpo_0000031 -->

    <owl:Class rdf:about="http://purl.obolibrary.org/obo/cpo_0000031">
        <rdfs:subClassOf rdf:resource="http://www.geneontology.org/formats/oboInOwl#ObsoleteClass"/>
        <obo:IAO_0000115 xml:lang="en">A precondition that allows for the possibility of a proximal outcome</obo:IAO_0000115>
        <obo:IAO_0000117 xml:lang="en">Cooper Stansbury</obo:IAO_0000117>
        <obo:IAO_0000119 xml:lang="en">Lewis CC, Klasnja P, Powell BJ, Lyon AR, Tuzzio L, Jones S, et al. From Classification to Causality: Advancing Understanding of Mechanisms of Change in Implementation Science. Front Public Health [Internet]. 2018 [cited 2018 Jun 6];6. Available from: https://www.frontiersin.org/articles/10.3389/fpubh.2018.00136/full</obo:IAO_0000119>
        <rdfs:label rdf:datatype="http://www.w3.org/2001/XMLSchema#string">obsolete precondition for proximal outcome</rdfs:label>
        <owl:deprecated rdf:datatype="http://www.w3.org/2001/XMLSchema#boolean">true</owl:deprecated>
    </owl:Class>
    


    <!-- http://purl.obolibrary.org/obo/cpo_0000032 -->

    <owl:Class rdf:about="http://purl.obolibrary.org/obo/cpo_0000032">
        <rdfs:subClassOf rdf:resource="http://www.geneontology.org/formats/oboInOwl#ObsoleteClass"/>
        <obo:IAO_0000115 xml:lang="en">A mechanism that affects mental representations of outcomes or end states that an individual wants to achieve.</obo:IAO_0000115>
        <obo:IAO_0000117 xml:lang="en">Cooper Stansbury</obo:IAO_0000117>
        <obo:IAO_0000119 xml:lang="en">Cane J, O’Connor D, Michie S. Validation of the theoretical domains framework for use in behaviour change and implementation research. Implementation Science. 2012 Apr 24;7:37.</obo:IAO_0000119>
        <rdfs:label rdf:datatype="http://www.w3.org/2001/XMLSchema#string">obsolete act on goal</rdfs:label>
        <owl:deprecated rdf:datatype="http://www.w3.org/2001/XMLSchema#boolean">true</owl:deprecated>
    </owl:Class>
    


    <!-- http://purl.obolibrary.org/obo/cpo_0000033 -->

    <owl:Class rdf:about="http://purl.obolibrary.org/obo/cpo_0000033">
        <rdfs:subClassOf rdf:resource="http://www.geneontology.org/formats/oboInOwl#ObsoleteClass"/>
        <obo:IAO_0000115 xml:lang="en">A mechanism that affects an awareness of the existence of something.</obo:IAO_0000115>
        <obo:IAO_0000117 xml:lang="en">Cooper Stansbury</obo:IAO_0000117>
        <obo:IAO_0000119 xml:lang="en">Cane J, O’Connor D, Michie S. Validation of the theoretical domains framework for use in behaviour change and implementation research. Implementation Science. 2012 Apr 24;7:37.</obo:IAO_0000119>
        <rdfs:label rdf:datatype="http://www.w3.org/2001/XMLSchema#string">obsolete act on knowledge</rdfs:label>
        <owl:deprecated rdf:datatype="http://www.w3.org/2001/XMLSchema#boolean">true</owl:deprecated>
    </owl:Class>
    


    <!-- http://purl.obolibrary.org/obo/cpo_0000034 -->

    <owl:Class rdf:about="http://purl.obolibrary.org/obo/cpo_0000034">
        <rdfs:subClassOf rdf:resource="http://www.geneontology.org/formats/oboInOwl#ObsoleteClass"/>
        <obo:IAO_0000115 xml:lang="en">A mechanism that affects a conscious decision to perform a behaviour or a resolve to act in a certain way.</obo:IAO_0000115>
        <obo:IAO_0000117 xml:lang="en">Cooper Stansbury</obo:IAO_0000117>
        <obo:IAO_0000119 xml:lang="en">Cane J, O’Connor D, Michie S. Validation of the theoretical domains framework for use in behaviour change and implementation research. Implementation Science. 2012 Apr 24;7:37.</obo:IAO_0000119>
        <obo:IAO_0000232 xml:lang="en">This was adapted from the category &apos;intention&apos; in the cited source. The authors list &apos;intrinic motivation&apos; under the category of intention. This needed to be revisited.</obo:IAO_0000232>
        <rdfs:label rdf:datatype="http://www.w3.org/2001/XMLSchema#string">obsolete act on motivation</rdfs:label>
        <owl:deprecated rdf:datatype="http://www.w3.org/2001/XMLSchema#boolean">true</owl:deprecated>
    </owl:Class>
    


    <!-- http://purl.obolibrary.org/obo/cpo_0000035 -->

    <owl:Class rdf:about="http://purl.obolibrary.org/obo/cpo_0000035">
        <rdfs:subClassOf rdf:resource="http://www.geneontology.org/formats/oboInOwl#ObsoleteClass"/>
        <obo:IAO_0000115 xml:lang="en">A moderator that is a sensitivity of the intended recipient of an intevention towards gain and pleasure</obo:IAO_0000115>
        <obo:IAO_0000117 xml:lang="en">Cooper Stansbury</obo:IAO_0000117>
        <obo:IAO_0000119 xml:lang="en">source needed</obo:IAO_0000119>
        <rdfs:label rdf:datatype="http://www.w3.org/2001/XMLSchema#string">obsolete promotion focus</rdfs:label>
        <owl:deprecated rdf:datatype="http://www.w3.org/2001/XMLSchema#boolean">true</owl:deprecated>
    </owl:Class>
    


    <!-- http://purl.obolibrary.org/obo/cpo_0000036 -->

    <owl:Class rdf:about="http://purl.obolibrary.org/obo/cpo_0000036">
        <rdfs:subClassOf rdf:resource="http://www.geneontology.org/formats/oboInOwl#ObsoleteClass"/>
        <obo:IAO_0000115 xml:lang="en">A moderator that is a sensitivity of the intended recipient of an intevention towards loss and avoidance of pain.</obo:IAO_0000115>
        <obo:IAO_0000117 xml:lang="en">Cooper Stansbury</obo:IAO_0000117>
        <obo:IAO_0000119 xml:lang="en">source needed</obo:IAO_0000119>
        <rdfs:label rdf:datatype="http://www.w3.org/2001/XMLSchema#string">obsolete prevention focus</rdfs:label>
        <owl:deprecated rdf:datatype="http://www.w3.org/2001/XMLSchema#boolean">true</owl:deprecated>
    </owl:Class>
    


    <!-- http://purl.obolibrary.org/obo/cpo_0000037 -->

    <owl:Class rdf:about="http://purl.obolibrary.org/obo/cpo_0000037">
        <rdfs:subClassOf rdf:resource="http://www.geneontology.org/formats/oboInOwl#ObsoleteClass"/>
        <obo:IAO_0000115 xml:lang="en">A moderator that is a method of presenting information that is intended to affect an intended reciepients&apos;s perception of gain or opporunity.</obo:IAO_0000115>
        <obo:IAO_0000117 xml:lang="en">Cooper Stansbury</obo:IAO_0000117>
        <obo:IAO_0000119 xml:lang="en">source needed</obo:IAO_0000119>
        <rdfs:label rdf:datatype="http://www.w3.org/2001/XMLSchema#string">obsolete promotion framing</rdfs:label>
        <owl:deprecated rdf:datatype="http://www.w3.org/2001/XMLSchema#boolean">true</owl:deprecated>
    </owl:Class>
    


    <!-- http://purl.obolibrary.org/obo/cpo_0000038 -->

    <owl:Class rdf:about="http://purl.obolibrary.org/obo/cpo_0000038">
        <rdfs:subClassOf rdf:resource="http://www.geneontology.org/formats/oboInOwl#ObsoleteClass"/>
        <obo:IAO_0000115 xml:lang="en">A moderator that is a method of presenting information that is intended to affect an intended reciepients&apos;s perception of loss or risk</obo:IAO_0000115>
        <obo:IAO_0000117 xml:lang="en">Cooper Stansbury</obo:IAO_0000117>
        <obo:IAO_0000119 xml:lang="en">source needed</obo:IAO_0000119>
        <rdfs:label rdf:datatype="http://www.w3.org/2001/XMLSchema#string">obsolete prevention framing</rdfs:label>
        <owl:deprecated rdf:datatype="http://www.w3.org/2001/XMLSchema#boolean">true</owl:deprecated>
    </owl:Class>
    


    <!-- http://purl.obolibrary.org/obo/cpo_0000039 -->

    <owl:Class rdf:about="http://purl.obolibrary.org/obo/cpo_0000039">
        <rdfs:subClassOf rdf:resource="http://www.geneontology.org/formats/oboInOwl#ObsoleteClass"/>
        <obo:IAO_0000115 xml:lang="en">An organizational moderator which is a method of presenting information that is intended to affect the influence of an implementation strategy.</obo:IAO_0000115>
        <obo:IAO_0000117 xml:lang="en">Cooper Stansbury</obo:IAO_0000117>
        <obo:IAO_0000119 xml:lang="en">source needed</obo:IAO_0000119>
        <rdfs:label rdf:datatype="http://www.w3.org/2001/XMLSchema#string">obsolete message framing</rdfs:label>
        <owl:deprecated rdf:datatype="http://www.w3.org/2001/XMLSchema#boolean">true</owl:deprecated>
    </owl:Class>
    


    <!-- http://purl.obolibrary.org/obo/cpo_0000040 -->

    <owl:Class rdf:about="http://purl.obolibrary.org/obo/cpo_0000040">
        <rdfs:subClassOf rdf:resource="http://www.geneontology.org/formats/oboInOwl#ObsoleteClass"/>
        <obo:IAO_0000117 xml:lang="en">Cooper Stansbury</obo:IAO_0000117>
        <rdfs:label rdf:datatype="http://www.w3.org/2001/XMLSchema#string">obsolete performance precondition</rdfs:label>
        <owl:deprecated rdf:datatype="http://www.w3.org/2001/XMLSchema#boolean">true</owl:deprecated>
    </owl:Class>
    


    <!-- http://purl.obolibrary.org/obo/cpo_0000041 -->

    <owl:Class rdf:about="http://purl.obolibrary.org/obo/cpo_0000041">
        <rdfs:subClassOf rdf:resource="http://www.geneontology.org/formats/oboInOwl#ObsoleteClass"/>
        <obo:IAO_0000117 xml:lang="en">Cooper Stansbury</obo:IAO_0000117>
        <rdfs:label rdf:datatype="http://www.w3.org/2001/XMLSchema#string">obsolete high performance - downward trend</rdfs:label>
        <owl:deprecated rdf:datatype="http://www.w3.org/2001/XMLSchema#boolean">true</owl:deprecated>
    </owl:Class>
    


    <!-- http://purl.obolibrary.org/obo/cpo_0000042 -->

    <owl:Class rdf:about="http://purl.obolibrary.org/obo/cpo_0000042">
        <rdfs:subClassOf rdf:resource="http://www.geneontology.org/formats/oboInOwl#ObsoleteClass"/>
        <obo:IAO_0000117 xml:lang="en">Cooper Stansbury</obo:IAO_0000117>
        <rdfs:label rdf:datatype="http://www.w3.org/2001/XMLSchema#string">obsolete high performance - stable</rdfs:label>
        <owl:deprecated rdf:datatype="http://www.w3.org/2001/XMLSchema#boolean">true</owl:deprecated>
    </owl:Class>
    


    <!-- http://purl.obolibrary.org/obo/cpo_0000043 -->

    <owl:Class rdf:about="http://purl.obolibrary.org/obo/cpo_0000043">
        <rdfs:subClassOf rdf:resource="http://www.geneontology.org/formats/oboInOwl#ObsoleteClass"/>
        <obo:IAO_0000117 xml:lang="en">Cooper Stansbury</obo:IAO_0000117>
        <rdfs:label rdf:datatype="http://www.w3.org/2001/XMLSchema#string">obsolete high performance - upward trend</rdfs:label>
        <owl:deprecated rdf:datatype="http://www.w3.org/2001/XMLSchema#boolean">true</owl:deprecated>
    </owl:Class>
    


    <!-- http://purl.obolibrary.org/obo/cpo_0000044 -->

    <owl:Class rdf:about="http://purl.obolibrary.org/obo/cpo_0000044">
        <rdfs:subClassOf rdf:resource="http://www.geneontology.org/formats/oboInOwl#ObsoleteClass"/>
        <obo:IAO_0000117 xml:lang="en">Cooper Stansbury</obo:IAO_0000117>
        <rdfs:label rdf:datatype="http://www.w3.org/2001/XMLSchema#string">obsolete low performance - downward trend</rdfs:label>
        <owl:deprecated rdf:datatype="http://www.w3.org/2001/XMLSchema#boolean">true</owl:deprecated>
    </owl:Class>
    


    <!-- http://purl.obolibrary.org/obo/cpo_0000045 -->

    <owl:Class rdf:about="http://purl.obolibrary.org/obo/cpo_0000045">
        <rdfs:subClassOf rdf:resource="http://www.geneontology.org/formats/oboInOwl#ObsoleteClass"/>
        <obo:IAO_0000117 xml:lang="en">Cooper Stansbury</obo:IAO_0000117>
        <rdfs:label rdf:datatype="http://www.w3.org/2001/XMLSchema#string">obsolete low performance - stable</rdfs:label>
        <owl:deprecated rdf:datatype="http://www.w3.org/2001/XMLSchema#boolean">true</owl:deprecated>
    </owl:Class>
    


    <!-- http://purl.obolibrary.org/obo/cpo_0000046 -->

    <owl:Class rdf:about="http://purl.obolibrary.org/obo/cpo_0000046">
        <rdfs:subClassOf rdf:resource="http://www.geneontology.org/formats/oboInOwl#ObsoleteClass"/>
        <obo:IAO_0000117 xml:lang="en">Cooper Stansbury</obo:IAO_0000117>
        <rdfs:label rdf:datatype="http://www.w3.org/2001/XMLSchema#string">obsolete low performance - upward trend</rdfs:label>
        <owl:deprecated rdf:datatype="http://www.w3.org/2001/XMLSchema#boolean">true</owl:deprecated>
    </owl:Class>
    


    <!-- http://purl.obolibrary.org/obo/cpo_0000047 -->

    <owl:Class rdf:about="http://purl.obolibrary.org/obo/cpo_0000047">
        <rdfs:subClassOf rdf:resource="http://www.geneontology.org/formats/oboInOwl#ObsoleteClass"/>
        <obo:IAO_0000117 xml:lang="en">Cooper Stansbury</obo:IAO_0000117>
        <rdfs:label rdf:datatype="http://www.w3.org/2001/XMLSchema#string">obsolete top performer</rdfs:label>
        <owl:deprecated rdf:datatype="http://www.w3.org/2001/XMLSchema#boolean">true</owl:deprecated>
    </owl:Class>
    


    <!-- http://purl.obolibrary.org/obo/cpo_0000050 -->

    <owl:Class rdf:about="http://purl.obolibrary.org/obo/cpo_0000050">
        <rdfs:subClassOf rdf:resource="http://www.geneontology.org/formats/oboInOwl#ObsoleteClass"/>
        <obo:IAO_0000115 xml:lang="en">A role inhering in a Homo sapiens which is realized in the process of receiving feedback during an intervention.</obo:IAO_0000115>
        <obo:IAO_0000117 xml:lang="en">Cooper Stansbury</obo:IAO_0000117>
        <obo:IAO_0000119 xml:lang="en">Needed.</obo:IAO_0000119>
        <rdfs:label rdf:datatype="http://www.w3.org/2001/XMLSchema#string">obsolete recipient role</rdfs:label>
        <owl:deprecated rdf:datatype="http://www.w3.org/2001/XMLSchema#boolean">true</owl:deprecated>
    </owl:Class>
    


    <!-- http://purl.obolibrary.org/obo/cpo_0000052 -->

    <owl:Class rdf:about="http://purl.obolibrary.org/obo/cpo_0000052">
        <rdfs:subClassOf rdf:resource="http://www.geneontology.org/formats/oboInOwl#ObsoleteClass"/>
        <obo:IAO_0000115 xml:lang="en">A process which affects an intervention outcome or variability of an intervention outcome.</obo:IAO_0000115>
        <obo:IAO_0000117 xml:lang="en">Cooper Stansbury</obo:IAO_0000117>
        <obo:IAO_0000119 xml:lang="en">Lewis CC, Klasnja P, Powell BJ, Lyon AR, Tuzzio L, Jones S, et al. From Classification to Causality: Advancing Understanding of Mechanisms of Change in Implementation Science. Front Public Health [Internet]. 2018 [cited 2018 Jun 6];6. Available from: https://www.frontiersin.org/articles/10.3389/fpubh.2018.00136/full</obo:IAO_0000119>
        <rdfs:label rdf:datatype="http://www.w3.org/2001/XMLSchema#string">obsolete contextual factor</rdfs:label>
        <owl:deprecated rdf:datatype="http://www.w3.org/2001/XMLSchema#boolean">true</owl:deprecated>
    </owl:Class>
    


    <!-- http://purl.obolibrary.org/obo/cpo_0000053 -->

    <owl:Class rdf:about="http://purl.obolibrary.org/obo/cpo_0000053">
        <rdfs:subClassOf rdf:resource="http://purl.obolibrary.org/obo/IAO_0000104"/>
        <obo:IAO_0000115 xml:lang="en">A plan specification that is designed to change specified behaviour patterns that may be used in an intervention.</obo:IAO_0000115>
        <obo:IAO_0000117 xml:lang="en">Cooper Stansbury</obo:IAO_0000117>
        <obo:IAO_0000119 xml:lang="en">Michie S, Stralen MMV, West R. The behaviour change wheel: A new method for characterising and designing behaviour change interventions. Implementation Science. 2011;6(1).</obo:IAO_0000119>
        <rdfs:label xml:lang="en">candidate intervention</rdfs:label>
    </owl:Class>
</rdf:RDF>



<!-- Generated by the OWL API (version 1.1.0) https://github.com/owlcs/owlapi -->

